/inti/privil/speedup!

AbstractPlatform/Types.bpl
@@ -147,23 +147,19 @@ axiom (forall o : tap_proof_op_t ::
         o == tap_proof_op_pause     ||
         o == tap_proof_op_release   ||
         o == tap_proof_op_block);
+        
 function tap_proof_op_valid(o : tap_proof_op_t) : bool 
 {
-    // o == tap_proof_op_compute   || o == tap_proof_op_destroy   ||
-    // o == tap_proof_op_enter     || o == tap_proof_op_exit      ||
-    // o == tap_proof_op_launch    || o == tap_proof_op_resume    ||
-    // o == tap_proof_op_pause     || o == tap_proof_op_release   ||
-    // o == tap_proof_op_block
-    false
-    // o == tap_proof_op_compute    
-    // o == tap_proof_op_destroy   
-    // o == tap_proof_op_enter     
-    // o == tap_proof_op_exit      
-    // o == tap_proof_op_launch    
-    // o == tap_proof_op_resume    
-    // o == tap_proof_op_pause     
-    // o == tap_proof_op_release   
-    // o == tap_proof_op_block
+    // false
+    o == tap_proof_op_compute ||    
+    o == tap_proof_op_destroy ||   
+    o == tap_proof_op_enter   ||   
+    o == tap_proof_op_exit    ||   
+    o == tap_proof_op_launch  ||  
+    o == tap_proof_op_resume  ||
+    o == tap_proof_op_pause   ||
+    o == tap_proof_op_release ||
+    o == tap_proof_op_block
 }
 
 function tap_proof_op_valid_in_enclave(o : tap_proof_op_t) : bool
@@ -174,16 +170,18 @@ function tap_proof_op_valid_in_enclave(o : tap_proof_op_t) : bool
     // o == tap_proof_op_exit      
 }
 
+/* proved: exit pause launch resume destroy */
+/* todo: compute enter resume */
 function tap_proof_op_valid_in_privileged (o : tap_proof_op_t) : bool
 {
     // o == tap_proof_op_compute   || o == tap_proof_op_destroy   ||
     // o == tap_proof_op_enter     || o == tap_proof_op_exit      ||
     // o == tap_proof_op_launch    || o == tap_proof_op_resume    ||
     // o == tap_proof_op_pause     
-    // false
+    false
     // o == tap_proof_op_compute   
     // o == tap_proof_op_destroy   
-    o == tap_proof_op_enter     
+    // o == tap_proof_op_enter     
     // o == tap_proof_op_exit      
     // o == tap_proof_op_launch    
     // o == tap_proof_op_resume    
